

Modified Power Series Solutions

ODE solutions are not always "smooth," and may not be resolved by a power series.

Euler's
Eqn.

$$x^2 u''(x) + ax u'(x) + bu(x) = 0$$

\uparrow $= 0$ at origin

The origin is a singular point of this ODE.

$$rx^{r-1}, r(r-1)x^{r-2}$$

$$\tilde{u}(x) = x^r \Rightarrow \underbrace{(r(r-1) + ar + b)}_{r^2 + (a-1)r + b = 0} \tilde{u}(x) = 0$$

$$r_{\pm} = \frac{1}{2} (1 - a \pm \sqrt{(1-a)^2 - 4b})$$

Solutions are not always smooth! E.g.



$$u(x) = c_1 1 + c_2 x^{-1/2} \quad (a = 1/2, b = -1/2)$$

\uparrow \uparrow
two lin. indep.



$$u(x) = c_1 x^{-1} + c_2 x^{-2} \quad (a = 5, b = 2)$$

The singularities is determined by the indicial eqn.

$$r^2 + ar + b = 0$$

$$(r - r_+)(r - r_-) = 0 \Rightarrow r_+ \neq r_-$$

$x^r \Rightarrow$ If $\text{Re}(r) \geq 0$, then the soln is bdd at $x=0$.

\Rightarrow If $\text{Im}(r) \neq 0$, solutions oscillate

\Rightarrow Repeated roots, 2nd solution has a log term

$$u(x) = c_1 x^r + c_2 x^r \log x$$

Modified Power Series

Idea: Modify basis set to "factor" out the singular behavior:

$$\{1, x, \dots, x^N\} \Rightarrow \begin{matrix} x^r & 1 & x^r x & & x^r x^N \\ \{x^r, & x^{r+1}, & \dots, & x^{r+N}\} \end{matrix}$$

Equivalently, use a power series ansatz with singular factor

$$\tilde{u}(x) = \underset{\substack{\uparrow \\ \text{singular} \\ \text{part}}}{x^r} \sum_{n=0}^{\infty} \underset{\substack{\uparrow \\ \text{smooth} \\ \text{part}}}{a_n} x^n$$

Need to find power series coeffs & exponent.

Example: $x^2 u''(x) + 4xu'(x) + (x^2 + 2)u(x) = 0$
 $\hat{=}$ singular point at $x=0$

$$2u(x) = 2x^r \sum_{n=0}^{\infty} a_n x^n \quad | \quad x^2 u(x) = \sum_{n=0}^{\infty} a_n x^{n+r+2}$$

$$= \sum_{n=0}^{\infty} 2a_n x^{n+r}$$

$$u'(x) = \sum_{n=0}^{\infty} (n+r) a_n x^{n+r-1}$$

$$4xu'(x) = \sum_{n=0}^{\infty} 4(n+r) a_n x^{n+r}$$

$$u''(x) = \sum_{n=0}^{\infty} (n+r)(n+r-1) a_n x^{n+r-2}$$

$$x^2 u''(x) = \sum_{n=0}^{\infty} (n+r)(n+r-1) a_n x^{n+r}$$

\Rightarrow Match coeffs of x^{n+r} ($n \geq 0$)

	coeffs of x^r	x^{r+1}	x^{r+2}	x^{r+n}
$x^2 u''$	$r(r-1)a_0$	$(r+1)ra_1$	$(r+2)(r+1)a_2$	$(n+r)(n+r-1)a_n$
$4xu'$	$4ra_0$	$4(r+1)a_1$	$4(r+2)a_2$	$4(n+r)a_n$
$x^2 u$	0	0	a_0	a_{n-2}
$2u$	$2a_0$	$2a_1$	$2a_2$	$2a_n$
(RHS)	0	0	0	0

depend on r !

$$\begin{bmatrix} a_0 \\ a_1 \\ \vdots \end{bmatrix} = \begin{bmatrix} 0 \\ 0 \\ \vdots \end{bmatrix}$$

$$\begin{bmatrix} & & \\ & & \\ & & \end{bmatrix} \begin{bmatrix} a_n \\ \vdots \\ a_1 \\ a_0 \end{bmatrix} = \begin{bmatrix} 0 \\ \vdots \\ 0 \end{bmatrix}$$

$$L(r) \underline{a} = \underline{0} \quad (\text{nonlinear eigenvalue problem})$$

$$(L - \rho(r)I) \underline{a} = \underline{0}$$

$$\underbrace{(r(r-1) + 4r + 2)}_{=0} a_0 = 0$$

$$r^2 + 3r + 2 = 0 \Rightarrow (r+2)(r+1) = 0$$

$$r = -1 \text{ and } r = -2$$

$$\tilde{u}_+(x) = x^{-1} \sum_{n=0}^{\infty} a_n x^n \quad \tilde{u}_-(x) = x^{-2} \sum_{n=0}^{\infty} b_n x^n$$

$$r = -1 \Rightarrow a_n = -\frac{1}{n(n+1)} a_{n-2} \quad a_0 \text{ free, } a_1 = 0$$

$$a_n = \begin{cases} \frac{(-1)^{n/2}}{(n+1)!} a_0, & n \text{ even} \\ 0, & n \text{ odd} \end{cases}$$

$$m = \frac{n}{2}$$

$$\tilde{u}_+(x) = a_0 x^{-1} \sum_{m=0}^{\infty} \frac{(-1)^m}{(2m+1)!} x^{2m}$$

$$= a_0 x^{-2} \left(x - \frac{x^3}{3!} + \frac{x^5}{5!} - \dots \right)$$

$$= a_0 \frac{\sin x}{x^2} \quad \Leftarrow \text{singular at } x=0$$

Fuchs's Theorem

$$(*) \quad u'' + f(x)u' + g(x)u = 0$$

Idea: $x^2 u'' + axu' + bu = 0 \Rightarrow u'' + \frac{a}{x} u' + \frac{b}{x^2} u = 0$

Thm: If $xf(x)$ and $x^2g(x)$ have convergent power series at $x=0$, then $(*)$ has either

a) 2 Lin. Indep. solutions of form

$$u_{\pm}(x) = x^{r_{\pm}} \sum_{n=0}^{\infty} a_n^{\pm} x^n$$

b) 1 Modified power series soln.

$s_1(x)$ and another lin indep. soln of form $s_1(x) \log(x) + s_2(x)$.